ccs/EquivalenceDO.v
@@ -1,0 +1,963 @@
+(* begin hide *)
+From Coq Require Import Morphisms.
+
+From ITree Require Import
+     ITree
+     Eq.Eq
+     Events.Exception
+     ITreeFacts.
+
+From CCS Require Import
+     PropT
+     Syntax
+     Utils
+     Operational
+     Denotational
+.
+Import ITreeNotations.
+Open Scope itree.
+Import CCSNotations.
+Import DenNotations.
+Open Scope ccs_scope.
+
+From Paco Require Import paco.
+From Coq Require Import Morphisms.
+(* end hide *)
+
+Section Inversion_Lemma.
+
+  (* TODO: Push some stuff in the itree library *)
+
+  Context {E : Type -> Type} {R1 R2 : Type} (RR : R1 -> R2 -> Prop).
+
+  Lemma eqitree_inv_Tau_r (t : itree E R1) t' :
+    eq_itree RR t (Tau t') -> exists t0, observe t = TauF t0 /\ eq_itree RR t0 t'.
+  Proof.
+    intros.
+    punfold H.
+    inv H;
+      try inv CHECK;
+      pclearbot;
+      eauto.
+  Qed.
+
+  Lemma eqitree_inv_Tau_l (t : itree E R1) t' :
+    eq_itree RR (Tau t) t' -> exists t0, observe t' = TauF t0 /\ eq_itree RR t t0.
+  Proof.
+    intros; punfold H; inv H; try inv CHECK; pclearbot; eauto.
+  Qed.
+
+  Lemma eqitree_inv_Ret_r (t : itree E R1) r :
+    eq_itree RR t (Ret r) -> exists r', RR r' r /\ observe t = RetF r'.
+  Proof.
+    intros; punfold H; inv H; try inv CHECK; eauto.
+  Qed.
+
+  Lemma eqitree_inv_Ret_l (t : itree E R2) r :
+    eq_itree RR (Ret r) t -> exists r', RR r r' /\ observe t = RetF r'.
+  Proof.
+    intros; punfold H; inv H; try inv CHECK; eauto.
+  Qed.
+
+  Lemma eqitF_inv_VisF_l {b1 b2 vclo sim}
+    X1 (e1 : E X1) (k1 : X1 -> _) t2 :
+     eqitF RR b1 b2 vclo sim (VisF e1 k1) t2 ->
+     (exists k2, t2 = VisF e1 k2 /\ forall v, vclo sim (k1 v) (k2 v)) \/
+     (b2 = true /\ exists t2', t2 = TauF t2' /\ eqitF RR b1 b2 vclo sim  (VisF e1 k1) (observe t2')).
+  Proof.
+    refine (fun H =>
+      match H in eqitF _ _ _ _ _ t1 _ return
+      match t1 return Prop with
+      | VisF e1 k1 => _
+      | _ => True
+      end
+    with
+    | EqVis _ _ _ _ _ _ _ _ _ => _
+    | _ => _
+    end); try exact I.
+    - left; eauto.
+    - destruct i; eauto.
+  Qed.
+
+  Lemma eqitree_inv_Vis_r {U} (t : itree E R1) (e : E U) (k : U -> itree E R2) :
+    eq_itree RR t (Vis e k) -> exists k', observe t = VisF e k' /\ forall u, eq_itree RR (k' u) (k u).
+  Proof.
+    intros.
+    punfold H.
+    apply eqitF_inv_VisF_r in H.
+    destruct H as [ [? [-> ?]] | [] ]; [ | discriminate ].
+    pclearbot.
+    eexists; split; eauto.
+  Qed.
+
+  Lemma eqitree_inv_Vis_l {U} (t : itree E R2) (e : E U) (k : U -> _) :
+    eq_itree RR (Vis e k) t -> exists k', observe t = VisF e k' /\ forall u, eq_itree RR (k u) (k' u).
+  Proof.
+    intros; punfold H; apply eqitF_inv_VisF_l in H.
+    destruct H as [ [? [-> ?]] | [] ]; [ | discriminate ].
+    pclearbot. eexists; split; eauto.
+  Qed.
+
+  Lemma eqitree_tau_ret_abs : forall (t : itree E R1) x,
+    eq_itree RR (Tau t) (Ret x) -> False.
+  Proof.
+    intros; edestruct @eqitree_inv_Tau_l as (? & abs &?); eauto; inv abs.
+  Qed.
+
+  Lemma eqitree_ret_tau_abs : forall (t : itree E R2) x,
+    eq_itree RR (Ret x) (Tau t) -> False.
+  Proof.
+   intros; edestruct @eqitree_inv_Tau_r as (? & abs &?); eauto; inv abs.
+  Qed.
+
+  Lemma eqitree_ret_vis_abs : forall {U} e (k : U -> itree E R2) x,
+    eq_itree RR (Ret x) (Vis e k) -> False.
+  Proof.
+   intros; edestruct @eqitree_inv_Vis_r as (? & abs &?); eauto; inv abs.
+  Qed.
+
+  Lemma eqitree_vis_ret_abs : forall {U} e (k : U -> itree E R1) x,
+    eq_itree RR (Vis e k) (Ret x) -> False.
+  Proof.
+    intros; edestruct @eqitree_inv_Vis_l as (? & abs &?); eauto; inv abs.
+  Qed.
+
+  Lemma eqitree_vis_tau_abs : forall {U} e (k : U -> itree E R1) t,
+    eq_itree RR (Vis e k) (Tau t) -> False.
+  Proof.
+    intros; edestruct @eqitree_inv_Vis_l as (? & abs &?); eauto; inv abs.
+  Qed.
+
+  Lemma eqitree_tau_vis_abs : forall {U} e (k : U -> itree E R2) t,
+    eq_itree RR (Tau t) (Vis e k) -> False.
+  Proof.
+    intros; edestruct @eqitree_inv_Vis_r as (? & abs &?); eauto; inv abs.
+  Qed.
+
+End Inversion_Lemma.
+
+Ltac inv_eqitree H :=
+  match type of H with
+  | eq_itree _ (Tau _) (Ret _)   => apply eqitree_tau_ret_abs in H; contradiction
+  | eq_itree _ (Ret _) (Tau _)   => apply eqitree_ret_tau_abs in H; contradiction
+  | eq_itree _ (Vis _ _) (Ret _) => apply eqitree_vis_ret_abs in H; contradiction
+  | eq_itree _ (Ret _) (Vis _ _) => apply eqitree_ret_vis_abs in H; contradiction
+  | eq_itree _ (Vis _ _) (Tau _) => apply eqitree_vis_tau_abs in H; contradiction
+  | eq_itree _ (Tau _) (Vis _ _) => apply eqitree_tau_vis_abs in H; contradiction
+  | eq_itree _ (Ret _) (Ret _)   => apply eqit_inv_Ret in H
+  | _ => idtac
+  end.
+ 
+Section EquivSem.
+
+  Notation step_op  := Operational.step.
+
+  (* Lifting the operational stepping over itrees to the syntax
+  via representation *)
+  Definition step_sem : term -> option action -> term -> Prop :=
+    fun t1 ma t2 => step_ccs (model t1) ma (model t2).
+
+  Notation "P '⊢' a '→sem' Q" := (step_sem P a Q) (at level 50).
+  Notation "P '⊢' a '→op'  Q" := (step_op P a Q)  (at level 50).
+
+  (* Lock-step bisimulation between terms and [ccs] *)
+  Variant bisimF bisim : term -> term -> Prop :=
+    _bisimF : forall P Q,
+      ((forall a P' (PStep : step_op P a P'),
+           exists Q', step_sem Q a Q' /\ bisim P' Q')
+       /\ (forall a Q' (QStep : step_sem Q a Q'),
+             exists P', step_op P a P' /\ bisim P' Q'))
+      -> bisimF bisim P Q.
+  Hint Constructors bisimF : core.
+
+  Definition bisim := paco2 bisimF bot2.
+  Hint Unfold bisim : core.
+
+  Lemma bisimF_mon : monotone2 bisimF.
+  Proof.
+    unfold monotone2.
+    intros.
+    inversion IN; subst.
+    destruct H as [StepOp StepSem].
+    econstructor.
+    split; intros.
+    - apply StepOp in PStep as [Q' [Sem2 RPQ]].
+      eauto.
+    - apply StepSem in QStep as [P' [Op2 RPQ]].
+      eauto.
+  Qed.
+  Hint Resolve bisimF_mon : paco.
+
+  Definition head_of_action a :=
+    match a with
+    | Some a => HAct a
+    | None => HSynch
+    end.
+
+  Inductive Returns_legacy {E} {A: Type} (a: A) : itree E A -> Prop :=
+  | Returns_legacyRet: forall t, t ≅ Ret a -> Returns_legacy a t
+  | Returns_legacyTau: forall t u, t ≅ Tau u -> Returns_legacy a u -> Returns_legacy a t
+  | Returns_legacyVis: forall {X} (e: E X) (x: X) t k, t ≅ Vis e k -> Returns_legacy a (k x) -> Returns_legacy a t.
+
+  Inductive Returns {A: Type} (a: A) : ccsT A -> Prop :=
+  | ReturnsRet: forall t, t ≅ Ret a -> Returns a t
+  | ReturnsTau: forall t u, t ≅ Tau u -> Returns a u -> Returns a t
+  | ReturnsChoiceL: forall (t P Q: ccsT A),
+      t ≅ Vis (inl1 Plus) (fun b: bool => if b then P else Q) ->
+      Returns a P -> Returns a t
+  | ReturnsChoiceR: forall t P Q,
+      t ≅ Vis (inl1 Plus) (fun b: bool => if b then P else Q) ->
+      Returns a Q -> Returns a t
+  | ReturnsPara2L: forall t P Q,
+      t ≅ Vis (inl1 Sched2) (fun b: bool => if b then P else Q) ->
+      Returns a P -> Returns a t
+  | ReturnsPara2R: forall t P Q,
+      t ≅ Vis (inl1 Sched2) (fun b: bool => if b then P else Q) ->
+      Returns a Q -> Returns a t
+  | ReturnsPara3L: forall t P Q R,
+      t ≅ Vis (inl1 Sched3) (fun c => match c with
+                                   | Left => P
+                                   | Right => Q
+                                   | Synchronize => R
+                                   end) ->
+      Returns a P -> Returns a t
+  | ReturnsPara3R: forall t P Q R,
+      t ≅ Vis (inl1 Sched3) (fun c => match c with
+                                   | Left => P
+                                   | Right => Q
+                                   | Synchronize => R
+                                   end) ->
+      Returns a Q -> Returns a t
+  | ReturnsPara3S: forall t P Q R,
+      t ≅ Vis (inl1 Sched3) (fun c => match c with
+                                   | Left => P
+                                   | Right => Q
+                                   | Synchronize => R
+                                   end) ->
+      Returns a R -> Returns a t.
+
+  Inductive Finite {E X} : itree E X -> Prop :=
+  | FRet : forall R t (x: X), eq_itree R t (Ret x) -> Finite t
+  | FTau : forall R t P, eq_itree R t (Tau P) -> Finite P -> Finite t
+  | FVis {A} : forall R t (e: E A) k,
+      eq_itree R t (Vis e k) -> (forall x, Finite (k x)) -> Finite t.
+
+  Inductive FiniteSchedTree {X} : itree ccsE X -> Prop :=
+  | FSTRet : forall R t (x: X), eq_itree R t (Ret x) -> FiniteSchedTree t
+  | FSTTau : forall R t P, eq_itree R t (Tau P) -> FiniteSchedTree P -> FiniteSchedTree t
+  | FSTPlus : forall R t k,
+      eq_itree R t (b <- trigger Plus;; k b) ->
+      (forall b, FiniteSchedTree (k b)) ->
+      FiniteSchedTree t
+  | FSTSched2 : forall R t k,
+      eq_itree R t (b <- trigger Sched2;; k b) ->
+      (forall b, FiniteSchedTree (k b)) ->
+      FiniteSchedTree t
+  | FSTSched3 : forall R t k,
+      eq_itree R t (c <- trigger Sched3;; k c) ->
+      (forall c, FiniteSchedTree (k c)) ->
+      FiniteSchedTree t.
+
+  Lemma step_ccs_through_FST :
+    forall (t : ccsT head) (k : head -> ccs) (q : ccs) a hd,
+     FiniteSchedTree t ->
+     Returns_legacy hd t ->
+     k hd ⊢ a →ccs q ->
+     (hd <- t;; k hd) ⊢ a →ccs q.
+  Admitted.
+
+  Lemma step_ccs_through_FST_weak :
+    forall (t : ccsT head) (k : head -> ccs) (q : ccs) a,
+     FiniteSchedTree t ->
+     (forall hd, k hd ⊢ a →ccs q) ->
+     (hd <- t;; k hd) ⊢ a →ccs q.
+  Admitted.
+
+  Lemma step_ccs_is_returned_by_get_hd :
+    forall (p q : ccs) a,
+      p ⊢ a →ccs q ->
+      Returns_legacy (head_of_action a q) (get_hd p).
+  Admitted.
+
+  Lemma finite_get_hd_FST : forall (p : ccs),
+    Finite p ->
+    FiniteSchedTree (get_hd p).
+  Admitted.
+
+  Lemma model_finite : forall (P : term),
+    Finite ⟦P⟧.
+  Admitted.
+
+  Lemma op_involutive : forall a, op (op a) = a.
+  Proof.
+    intros []; reflexivity.
+  Qed. 
+
+  Lemma SumL_sem :
+    forall P a Q P',
+      P ⊢a→sem P' ->
+      P ⊕ Q ⊢a→sem P'.
+  Proof.
+    intros.
+    apply S_Plus_L with ⟦P⟧ ⟦Q⟧; auto; reflexivity.
+  Qed.
+
+  Lemma SumR_sem :
+    forall P a Q Q',
+      Q ⊢a→sem Q' ->
+      P ⊕ Q ⊢a→sem Q'.
+  Proof.
+    intros.
+    apply S_Plus_R with ⟦P⟧ ⟦Q⟧; auto; reflexivity.
+  Qed.
+
+ Lemma ParL_sem :
+    forall P a Q P',
+      P ⊢a→sem P' ->
+      P ∥ Q ⊢a→sem P' ∥ Q. 
+  Proof.
+    intros * STEP.
+    unfold step_sem in *.
+    cbn.
+    rewrite para_unfold.
+    apply step_ccs_through_FST with (head_of_action a ⟦P'⟧).
+    3:apply step_ccs_through_FST_weak.
+    * apply finite_get_hd_FST, model_finite.
+    * apply step_ccs_is_returned_by_get_hd; assumption.
+    * apply finite_get_hd_FST, model_finite.
+    * intros hd.
+      destruct hd eqn:EQHD, a eqn:EQa; cbn;
+        try (constructor; unfold act,synch; rewrite bind_trigger; reflexivity);
+        try (eapply S_Sched2_L; [constructor; unfold act,synch; rewrite bind_trigger; reflexivity | reflexivity]).
+        destruct (are_opposite a1 a0).
+        eapply S_Sched3_L; [constructor; unfold act; rewrite bind_trigger; reflexivity | reflexivity].
+        eapply S_Sched2_L; [constructor; unfold act; rewrite bind_trigger; reflexivity | reflexivity].
+  Qed.
+
+  Lemma ParR_sem :
+    forall P a Q Q',
+      Q ⊢a→sem Q' ->
+      P ∥ Q ⊢a→sem P ∥ Q'. 
+  Proof.
+    intros * STEP.
+    unfold step_sem in *.
+    cbn.
+    rewrite para_unfold.
+    apply step_ccs_through_FST_weak.
+    2:intros; apply step_ccs_through_FST with (head_of_action a ⟦Q'⟧).
+    * apply finite_get_hd_FST, model_finite.
+    * apply finite_get_hd_FST, model_finite.
+    * apply step_ccs_is_returned_by_get_hd; assumption.
+    * destruct hd eqn:EQHD, a eqn:EQa; cbn;
+        try (constructor; unfold act,synch; rewrite bind_trigger; reflexivity);
+        try (eapply S_Sched2_R; [constructor; unfold act,synch; rewrite bind_trigger; reflexivity | reflexivity]).
+        destruct (are_opposite a0 a1).
+        eapply S_Sched3_R; [constructor; unfold act,synch; rewrite bind_trigger; reflexivity | reflexivity].
+        eapply S_Sched2_R; [constructor; unfold act,synch; rewrite bind_trigger; reflexivity | reflexivity].
+  Qed.
+
+  Lemma ParS_sem :
+    forall P a Q P' Q',
+      P ⊢Some a→sem P' ->
+      Q ⊢Some (op a)→sem Q' ->
+      P ∥ Q ⊢None→sem P' ∥ Q'. 
+  Proof.
+    intros * STEP_P STEP_Q.
+    unfold step_sem in *.
+    cbn.
+    rewrite para_unfold.
+    apply step_ccs_through_FST with (head_of_action (Some a) ⟦P'⟧).
+    3:apply step_ccs_through_FST with (head_of_action (Some (op a)) ⟦Q'⟧).
+    * apply finite_get_hd_FST, model_finite.
+    * apply step_ccs_is_returned_by_get_hd; assumption.
+    * apply finite_get_hd_FST, model_finite.
+    * apply step_ccs_is_returned_by_get_hd; assumption.
+    * cbn. 
+      unfold are_opposite.
+      rewrite op_involutive, eqb_action_refl.
+      eapply S_Sched3_S; [constructor; unfold synch; rewrite bind_trigger; reflexivity | reflexivity].
+  Qed.
+
+  #[global] Instance restrict_eq_itree c : 
+      Proper (eq_itree eq ==> eq_itree eq) (restrict c).
+  Proof.
+    unfold restrict; do 2 red; intros * EQ; rewrite EQ; reflexivity.
+  Qed.
+
+  #[global] Instance restrict_eutt c : 
+      Proper (eutt eq ==> eutt eq) (restrict c).
+  Proof.
+    unfold restrict; do 2 red; intros * EQ; rewrite EQ; reflexivity.
+  Qed.
+
+  Lemma restrict_tau : forall c P,
+    restrict c (Tau P) ≅ Tau (restrict c P).
+  Proof.
+    unfold restrict; intros; rewrite interp_tau; reflexivity.
+  Qed. 
+
+  Lemma restrict_act : forall c P a,
+    use_channel c (Some a) = false ->
+    restrict c (act a;; P) ≈ act a;; restrict c P.
+  Proof.
+    unfold restrict, act; intros * NEQ.
+    rewrite interp_bind, interp_trigger.
+    cbn in *; destruct a; rewrite NEQ; reflexivity.
+  Qed. 
+
+  Lemma restrict_synch : forall c P,
+    use_channel c None = false ->
+    restrict c (synch;; P) ≈ synch;; restrict c P.
+  Proof.
+    unfold restrict, synch; intros * NEQ.
+    rewrite interp_bind, interp_trigger.
+    reflexivity.
+  Qed. 
+
+  Lemma restrict_plus : forall c L R,
+    restrict c (plus L R) ≈ plus (restrict c L) (restrict c R).
+  Proof.
+    unfold restrict, plus; intros *.
+    rewrite interp_bind, interp_trigger.
+    cbn.
+    apply eutt_eq_bind; intros []; reflexivity.
+  Qed. 
+
+  Lemma restrict_branch2 : forall c L R,
+    restrict c (branch2 L R) ≈ branch2 (restrict c L) (restrict c R).
+  Proof.
+    unfold restrict, branch2; intros *.
+    rewrite interp_bind, interp_trigger.
+    cbn.
+    apply eutt_eq_bind; intros []; reflexivity.
+  Qed. 
+
+  Lemma restrict_branch3 : forall c L R S,
+    restrict c (branch3 L R S) ≈ branch3 (restrict c L) (restrict c R) (restrict c S).
+  Proof.
+    unfold restrict, branch3; intros *.
+    rewrite interp_bind, interp_trigger.
+    cbn.
+    apply eutt_eq_bind; intros []; reflexivity.
+  Qed. 
+
+  Lemma Restrict_sem_aux :
+    forall P a c P',
+      use_channel c a = false ->
+      P ⊢a→ccs P' ->
+      restrict c P ⊢a→ccs restrict c P'.
+  Proof.
+    intros * NEQ STEP.
+    induction STEP; rewrite H.
+    - rewrite restrict_act; auto.
+      constructor; reflexivity.
+    - rewrite restrict_synch; auto. 
+      constructor; reflexivity.
+    - rewrite restrict_plus.
+      eapply S_Plus_L; eauto. 
+      reflexivity.
+    - rewrite restrict_plus.
+      eapply S_Plus_R; eauto.
+      reflexivity.
+    - rewrite restrict_branch2.
+      eapply S_Sched2_L; [| reflexivity].
+      eauto. 
+    - rewrite restrict_branch2.
+      eapply S_Sched2_R; [| reflexivity].
+      eauto. 
+    - rewrite restrict_branch3.
+      eapply S_Sched3_L; [| reflexivity].
+      eauto. 
+    - rewrite restrict_branch3.
+      eapply S_Sched3_R; [| reflexivity].
+      eauto. 
+    - rewrite restrict_branch3.
+      eapply S_Sched3_S; [| reflexivity].
+      eauto. 
+  Qed.
+
+  Lemma Restrict_sem :
+    forall P a c P',
+      use_channel c a = false ->
+      P ⊢a→sem P' ->
+      P ∖ c ⊢a→sem P' ∖ c.
+  Proof.
+    intros * NEQ STEP.
+    apply Restrict_sem_aux; auto.
+  Qed.    
+
+  Theorem model_complete :
+    forall P a Q, 
+      P ⊢a→op Q ->
+      P ⊢a→sem Q.
+  Proof.
+    intros * StepOp.
+    (* Lock-step simulation *)
+    induction StepOp;
+      try now constructor.
+    + apply SumL_sem; assumption. 
+
+    + apply SumR_sem; assumption. 
+      
+    + apply ParL_sem; assumption. 
+
+    + apply ParR_sem; assumption. 
+    
+    + eapply ParS_sem; eassumption. 
+       
+    + (* Restrict *)
+      apply Restrict_sem; assumption.
+
+  Qed.
+
+  Theorem model_correct :
+    forall P a Q, 
+      P ⊢a→sem Q ->
+      P ⊢a→op Q.
+  Proof.
+  Admitted.
+
+  Theorem model_correct_complete :
+    forall P, bisim P P.
+  Proof.
+    pcofix CIH.
+    intros P.
+    pfold.
+    econstructor.
+    split.
+
+    - (* The denotational side can simulate the operational semantics *)
+      intros a P' StepOp.
+      exists P'.
+      split; [| right; auto].
+      clear CIH r.
+      apply model_complete; auto.
+
+    - (* The operational side can simulate the denotational semantics *)
+      intros a P' StepSem.
+      exists P'; split; [| auto].
+      apply model_correct; auto.
+
+  Qed.
+
+  (* BEGIN PROOFS IN PROGRESS FOR THE ADMITTED LEMMAS ABOVE *)
+
+  Definition eq_head R : head -> head -> Prop :=
+    fun h1 h2 =>
+      match h1,h2 with
+      | HDone, HDone => True
+      | HSynch t1, HSynch t2 => eq_itree R t1 t2
+      | HAct a1 t1, HAct a2 t2 => a1 = a2 /\ eq_itree R t1 t2
+      | _, _ => False
+      end.
+  Hint Unfold eq_head : core.
+
+  Global Instance get_hd_eq_itree {R} :
+    Proper (eq_itree R ==> eq_itree (eq_head R)) get_hd.
+  Proof.
+    do 2 red.
+    ginit.
+    gcofix CIH.
+    intros * EQ.
+    punfold EQ.
+    setoid_rewrite get_hd_unfold.
+    induction EQ; try inv CHECK.
+    - gstep; constructor; reflexivity.
+    - gstep; pclearbot. constructor; auto with paco.
+    - gstep; pclearbot.
+      destruct e as [? | [? | [? | ?]]].
+      + constructor; red; auto with paco.
+      + destruct a; constructor; auto.
+      + destruct s; constructor; auto.
+      + constructor; auto.
+  Qed.
+
+  Lemma FST_means_Finite {X}: forall (P: itree ccsE X), FiniteSchedTree P -> Finite P.
+  Proof.
+    intros.
+    induction H.
+    - now apply FRet with R x.
+    - now apply FTau with R P.
+    - rewrite bind_trigger in H.
+      eapply FVis;
+        eauto.
+    - rewrite bind_trigger in H.
+      eapply FVis;
+        eauto.
+    - rewrite bind_trigger in H.
+      eapply FVis;
+        eauto.
+  Qed.
+
+  Global Instance Finite_eq_itree {E X} R :
+    Proper (eq_itree R ==> flip impl) (@Finite E X).
+  Proof.
+    do 4 red.
+    intros x y Cong Fin.
+    revert x Cong.
+    induction Fin;
+      intros.
+    - apply FRet with (rcompose R R0) x.
+      eapply eqit_trans;
+        eauto.
+    - apply eqitree_inv_Tau_r in H.
+      destruct H as [t' [Obs Cong']].
+      apply FTau with (rcompose R R0) P.
+      + eapply eqit_trans.
+        * apply Cong.
+        * rewrite itree_eta, Obs.
+          apply eqit_Tau.
+          apply Cong'.
+      + assumption.
+    - apply eqitree_inv_Vis_r in H.
+      destruct H as [t' [Obs Cong']].
+      eapply FVis.
+      + eapply eqit_trans.
+        * eauto.
+        * rewrite itree_eta, Obs.
+          apply eqit_Vis.
+          apply Cong'.
+      + assumption.
+  Qed.
+
+  Global Instance FST_eq_itree {X} R :
+    Proper (eq_itree R ==> flip impl) (@FiniteSchedTree X).
+  Proof.
+    do 4 red.
+    intros x y Cong Fin.
+    revert x Cong.
+    induction Fin;
+      intros.
+    - apply FSTRet with (rcompose R R0) x.
+      eapply eqit_trans;
+        eauto.
+    - apply eqitree_inv_Tau_r in H.
+      destruct H as [t' [Obs Cong']].
+      apply FSTTau with (rcompose R R0) P.
+      + eapply eqit_trans.
+        * eauto.
+        * rewrite itree_eta, Obs.
+          apply eqit_Tau.
+          apply Cong'.
+      + assumption.
+    - apply FSTPlus with (rcompose R R0) k.
+      + eapply eqit_trans;
+          eauto.
+      + assumption.
+    - apply FSTSched2 with (rcompose R R0) k.
+      + eapply eqit_trans;
+          eauto.
+      + assumption.
+    - apply FSTSched3 with (rcompose R R0) k.
+      + eapply eqit_trans;
+          eauto.
+      + assumption.
+  Qed.
+
+  Ltac break_match_goal :=
+    match goal with
+    | [ |- context [ match ?X with _ => _ end ] ] =>
+      match type of X with
+      | sumbool _ _ => destruct X
+      | _ => destruct X eqn:?
+      end
+    end.
+
+  Theorem finite_head : forall P, Finite P -> FiniteSchedTree (get_hd P).
+  Proof.
+    intros.
+    induction H.
+    - (* Ret *)
+      pose proof (get_hd_unfold (Ret x)) as Eq;
+        cbn in Eq.
+      apply FSTRet with (eq_head R) HDone.
+      apply get_hd_eq_itree in H.
+      now rewrite Eq in H.
+    - (* Tau *)
+      pose proof (get_hd_unfold (Tau P)) as Eq;
+        cbn in Eq.
+      rewrite H, Eq.
+      now apply FSTTau with eq (get_hd P).
+    - (* Vis *)
+      rewrite H.
+      rewrite get_hd_unfold; cbn.
+      break_match_goal.
+      + (* Vis NonDetE, special case *)
+        induction n;
+          [ apply FSTPlus with eq (fun x => get_hd (k x))
+          | apply FSTSched2 with eq (fun x => get_hd (k x))
+          | apply FSTSched3 with eq (fun x => get_hd (k x))];
+          (now rewrite bind_trigger || assumption).
+      + (* Vis anything else *)
+        repeat break_match_goal;
+          now eapply FSTRet.
+  Qed.
+
+  Lemma finite_bind {E X Y} : forall (t: itree E Y) (k: Y -> itree E X),
+      Finite t -> (forall y, Finite (k y)) -> Finite (y <- t;; k y).
+  Proof.
+    intros t k Fin.
+    induction Fin;
+      intros FinK.
+    - apply eqitree_inv_Ret_r in H as [r' [_ Eq]].
+      now rewrite unfold_bind, Eq.
+    - apply eqitree_inv_Tau_r in H as [t' [Eq Rel]].
+      rewrite unfold_bind, Eq.
+      eapply FTau.
+      + reflexivity.
+      + apply IHFin in FinK.
+        admit.
+    - apply eqitree_inv_Vis_r in H as [k' [Eq Rel]].
+      rewrite unfold_bind, Eq.
+      eapply FVis.
+      + reflexivity.
+      + cbn.
+        intros.
+        apply H1 with x in FinK.
+        admit.
+  Admitted.
+
+  Lemma finite_interp {E F X} : forall (h : Handler E F) (t : itree E X),
+      Finite t ->
+      (forall Y (e : E Y), Finite (h _ e)) ->
+      Finite (interp h t).
+  Proof.
+    intros h t FinT.
+    revert h.
+    induction FinT;
+      intros.
+    - apply eqitree_inv_Ret_r in H as [r' [_ Eq]].
+      rewrite unfold_interp;
+        unfold _interp;
+        rewrite Eq.
+      now apply FRet with eq r'.
+    - apply eqitree_inv_Tau_r in H as [t' [Eq Rel]].
+      rewrite unfold_interp;
+        unfold _interp;
+        rewrite Eq.
+      apply FTau with eq (interp h t').
+      + reflexivity.
+      + apply IHFinT in H0.
+        admit.
+    - apply eqitree_inv_Vis_r in H as [k' [Eq Rel]].
+      rewrite unfold_interp;
+        unfold _interp;
+        rewrite Eq.
+      apply finite_bind.
+      + apply H2.
+      + intro.
+        apply FTau with eq (interp h (k' y)).
+        * reflexivity.
+        * apply H1 with (x := y) in H2.
+          admit.
+  Admitted.
+
+(* In order to prove that : [forall P, finite (model P)],
+    we need to reason about the co-recursive call performed by para.
+    However, this call does not take place on immediately structurally smaller
+    arguments, whether on the syntactic level via model nor on the trees themselves.
+    One sensible first step is to introduce an intermediate result on [para]:
+    [forall t s, Finite t -> Finite s -> Finite (para t s)]
+    As mentionned above however, this is still not the panacea: [Finite] essentially
+    gives structural induction on your tree, but the call is still not structural.
+    Hence we probably need to introduce the size of finite trees and proceed by
+    strong induction on the sum of the sizes of both trees, which requires quite
+    a bit of boilerplate and work.
+*)
+
+  Theorem finite_model : forall P, Finite (model P).
+  Proof.
+    induction P;
+      cbn.
+    - (* 0 *)
+      unfold done.
+      now apply FRet with eq tt.
+    - (* a ⋅ P *)
+      unfold act.
+      rewrite bind_trigger.
+      now eapply FVis.
+    - (* para *)
+      rewrite para_unfold.
+      apply finite_bind.
+      + apply FST_means_Finite.
+        now apply finite_head.
+      + intro rP.
+        apply finite_bind.
+        * apply FST_means_Finite.
+          now apply finite_head.
+        * intro rQ.
+          destruct rP, rQ;
+            try assumption.
+          -- now apply FRet with eq tt. 
+          -- admit.
+          -- admit.
+          -- admit.
+          -- unfold branch2.
+             rewrite bind_trigger.
+             eapply FVis.
+             ++ reflexivity.
+             ++ intro.
+                cbn.
+                case_eq x; intro; subst.
+                ** eapply FVis.
+                   --- reflexivity.
+                   --- intros []; cbn.
+                       admit.
+                ** eapply FVis.
+                   --- reflexivity.
+                   --- intro; cbn.
+                       admit.
+          -- admit.
+          -- admit.
+          -- admit.
+          -- admit.
+    - (* plus *)
+      unfold plus.
+      rewrite bind_trigger.
+      eapply FVis.
+      + reflexivity.
+      + intro b.
+        case_eq b;
+          auto.
+    - (* restrict *)
+      apply finite_interp.
+      + assumption.
+      + admit.
+  Admitted.
+
+  Lemma get_hd_FST : forall P, FiniteSchedTree (get_hd (model P)).
+  Proof.
+    intros; eapply finite_head, finite_model.
+  Qed.
+
+  Lemma FST_prefix_can_step {X} : forall (t : ccsT X) (k : X -> ccs) a t',
+      FiniteSchedTree t ->
+      (forall x, step_ccs (k x) a t') ->
+      step_ccs (x <- t;; k x) a t'.
+  Proof.
+    intros.
+    induction H.
+    - apply eqitree_inv_Ret_r in H as [r' [_ Eq]].
+      now rewrite unfold_bind, Eq.
+    - apply eqitree_inv_Tau_r in H as [t0 [Eq Rel]].
+      rewrite unfold_bind, Eq.
+      rewrite tau_eutt.
+  Admitted.
+
+  Theorem step_ccs_get_hd_returns : forall P a P',
+      step_ccs P a P'
+      ->
+      Returns_legacy (head_of_action a P') (get_hd P).
+  Proof.
+    intros.
+    induction H.
+    - pose proof (get_hd_unfold (Tau P)) as Eq;
+        cbn in Eq.
+      (* rewrite <- H0 in Eq. *)
+  Admitted.
+
+  Theorem get_hd_means_step_deprecated : forall P a P',
+      Returns_legacy (head_of_action a P') (get_hd P)
+      <->
+      step_ccs P a P'.
+  Proof.
+    split; intros.
+    - (* Returns -> step :
+       * if a finite path exists in the [get_hd] tree, it
+       * can be used as a proof tree to justify a [step_ccs] *)
+      remember (head_of_action a P') as aP'.
+      remember (get_hd P) as head_P.
+      revert P Heqhead_P.
+      (* By induction on the path in the tree *)
+      induction H.
+      + (* [get_hd P] is a [Ret x], we derive information on the shape of P *)
+        intros; subst.
+        pose proof (itree_eta P) as EQ.
+        rewrite EQ.
+        apply get_hd_eq_itree in EQ.
+        rewrite H in EQ; clear H.
+        destruct (observe P).
+        * (* Can't be a Ret *)
+          rewrite get_hd_unfold in EQ; cbn in EQ.
+          inv_eqitree EQ.
+          destruct a; cbn in EQ; contradiction.
+        * (* Can't be a Tau *)
+          rewrite get_hd_unfold in EQ; cbn in EQ.
+          inv_eqitree EQ.
+        * rewrite get_hd_unfold in EQ; cbn in EQ.
+          destruct e; cbn; inv_eqitree EQ.
+          destruct s; cbn.
+          destruct a0; cbn; inv_eqitree EQ.
+          destruct a; cbn in EQ; try contradiction.
+          destruct EQ as [<- EQ].
+          constructor.
+          unfold act; rewrite bind_trigger; apply eqit_Vis; intros [].
+          symmetry; auto. 
+          (*
+          destruct s; cbn; inv_eqitree EQ.
+          destruct s; cbn; inv_eqitree EQ.
+          destruct a; cbn in EQ; try contradiction.
+          constructor.
+          rewrite bind_trigger; apply eqit_Vis; intros [].
+          symmetry; auto.
+          destruct a; cbn in EQ; contradiction.
+      + (* [get_hd] starts with a [Tau] *)
+        intros; subst.
+        pose proof (itree_eta P) as EQ.
+        rewrite EQ.
+        apply get_hd_eq_itree in EQ.
+        rewrite H in EQ; clear H.
+        destruct (observe P);
+          rewrite get_hd_unfold in EQ;
+          cbn in EQ;
+          inv_eqitree EQ.
+        * admit.
+        * destruct e; cbn in *; inv_eqitree EQ.
+          destruct s; cbn in *; inv_eqitree EQ.
+          destruct a0; cbn in *; inv_eqitree EQ.
+          destruct s; cbn in *; inv_eqitree EQ.
+          destruct s; cbn in *; inv_eqitree EQ.
+      (*
+        eapply S_Tau; [apply IHReturns_legacy |].
+        admit.
+        admit. *)
+      + intros; subst.
+        pose proof (itree_eta P) as EQ; rewrite EQ; apply get_hd_eq_itree in EQ.
+        rewrite H in EQ; clear H.
+        destruct (observe P); rewrite get_hd_unfold in EQ; cbn in EQ; inv_eqitree EQ.
+        destruct e0; cbn in *; inv_eqitree EQ.
+        * admit.
+        * destruct s; cbn in *; inv_eqitree EQ.
+          destruct a0; cbn in *; inv_eqitree EQ.
+          destruct s; cbn in *; inv_eqitree EQ.
+          destruct s; cbn in *; inv_eqitree EQ.
+   - (* Step -> Returns *)
+      induction H.
+      + admit.
+      + admit. *)
+  Admitted.
+
+  Theorem get_hd_always_returns : forall P, exists a k, Returns (head_of_action a k) (get_hd (model P)).
+  Proof.
+    induction P.
+    - simpl.
+  Admitted.
+
+    (* écrire :
+      prédicat finite
+      pour tout P, finite model P
+      finite P -> finite (get_hd P)
+
+     écrire (et prouver)
+      pour tout P, exists a k, Returns++ (a,k) (get_hd (model P))
+
+     réfléchir à comment écrire
+      ????
+      Returns++ (a,k) P -> step (c a) b Q -> step (P ;; c) b q
+      "si la deuxième moitié du para passe (wrt. step), la première devrait passer aussi parce que les get_hds sont finis"
+      ????
+     *)
+
+  Set Nested Proofs Allowed.
+
+End EquivSem.
